examples/dm4all/IOCurriedReadWrite.fst
@@ -1,0 +1,109 @@
+module IOCurriedReadWrite
+
+open FStar.List
+open FStar.WellFounded
+
+type input = int
+type output = int
+
+noeq
+type io a =
+  | Read    : (input -> io a) -> io a
+  | Write   : output -> io a -> io a
+  | Return  : a -> io a
+
+let return (a:Type u#a) (x:a) = Return x
+
+let rec bind (a : Type u#aa) (b : Type u#bb)
+         (l : io a) (k : a -> io b) : io b =
+  match l with
+  | Read f -> Read (fun i -> axiom1 f i; bind _ _ (f i) k)
+  | Write o k' -> Write o (bind _ _ k' k)
+  | Return v -> k v
+
+type event =
+  | Rd : input -> event
+  | Wr : output -> event
+
+let h_trace = list event
+let l_trace = list event
+
+let post a = a -> l_trace -> Type0
+(* flipping these arguments will break the gen_wps_for_free logic, FIXME *)
+let wpty a = h_trace -> post a -> Type0
+
+let return_wp (a:Type) (x:a) : wpty a =
+  fun h p -> p x []
+
+let bind_wp (_ : range) (a:Type) (b:Type) (w : wpty a) (kw : a -> wpty b) : wpty b =
+  fun h p -> w h (fun x l -> kw x (h @ l) (fun y l' -> p y (l @ l')))
+
+let rec interpretation #a (m : io a) (h : h_trace) (p : post a) : Type0 =
+  match m with
+  | Write o m -> interpretation m (h @ [Wr o]) (fun x l -> p x ((Wr o) :: l))
+  | Read f -> forall (i : input). (axiom1 f i ; interpretation (f i) (h @ [Rd i]) (fun x l -> p x ((Rd i) :: l)))
+  | Return x -> p x []
+
+total
+reifiable
+reflectable
+new_effect {
+  IO : a:Type -> Effect
+  with
+       repr      = io
+     ; return    = return
+     ; bind      = bind
+
+     ; wp_type   = wpty
+     ; return_wp = return_wp
+     ; bind_wp   = bind_wp
+
+     ; interp = interpretation
+}
+
+val read : unit -> IO int (fun h p -> forall x. p x [Rd x])
+let read () =
+    IO?.reflect (Read (fun i -> Return i))
+
+(* Keeping the log backwards, since otherwise the VCs are too contrived for z3.
+ * Likely something we should fix separately.. *)
+
+val write : o:int -> IO unit (fun h p -> p () [Wr o])
+let write i =
+    IO?.reflect (Write i (Return ()))
+
+open FStar.Tactics
+
+let test1 () : IO int (fun h p -> p 1 [Wr 2; Wr 3]) =
+  write 2;
+  write 3;
+  1
+
+let test2 () : IO int (fun h p -> forall i . p 1 [Wr 2; Rd i; Wr 3]) by (compute ()) =
+  write 2;
+  let x = read () in
+  write 3;
+  1
+
+effect Io (a:Type) (pre':h_trace -> Type0) (post':h_trace -> a -> l_trace -> Type0) =
+        IO a (fun h p -> pre' h /\ (forall r l . post' h r l ==> p r l))
+
+let test3 (i:int) 
+  : Io int (requires (fun h     -> exists h' h'' . h = h' @ (Rd i :: h''))) 
+           (ensures  (fun h x l -> exists x . l = [Wr i; Rd x; Wr x])) by (compute ()) =
+  write i;
+  let x = read () in
+  write x;
+  1
+
+let rec n_w_events (n:nat) (i:int) = 
+  if n = 0 
+  then []
+  else Wr i :: n_w_events (n - 1) i
+
+let rec test4 (n:nat) (i:int)
+  : Io unit (requires (fun _     -> True)) 
+            (ensures  (fun h x l -> l = n_w_events n i)) by (compute ()) = 
+  if n = 0
+  then ()
+  else (write i; test4 (n - 1) i)
